README.md
@@ -1,0 +1,11 @@
+# Challenges of verifying persistent data structures
+
+This is the repository for my semester project at EPFL Spring 2023. The project proposal, the final report, and the presentation slides can all be found at the top level. The file `FatNode.dfy` contains the partial verified implementation of the fat node method in Dafny. 
+
+The fat node method is introduced by Driscoll et al. and illustrated in [this paper](https://www.cs.cmu.edu/~sleator/papers/making-data-structures-persistent.pdf). Previously, I have written a seminar report on this paper that can be found [here](https://github.com/kumom/persistent-AVL-tree).
+
+Before reading the report or the slides, it is strongly encouraged to first play with [the visualization](https://kumom.io/persistent-bst) of the fat node method, where the source code can be found [here](https://github.com/kumom/persistent-tree-visualization). 
+
+After reading the report, you may be intrigued to inspect all the interesting snapshots we have collected. An easier way to navigate through these examples is to read [this blog article](https://kumom.io/articles/instability), but you can also directly check out different branches and search for `COMMENT` in the code to inspect the relevant part. Commits in the `main` branch are also interesting snapshots, although they are less representative and harder to understand.
+
+Comments and suggestions are welcomed and should be sent to my private gmail address (see my GitHub profile).
